\documentclass{ximera}

\input{../../../preamble.tex}


\author{Lee Wayand}

\begin{document}
\begin{exercise}


\begin{question}



Let 

\[
H(x) = 4 2^{5x - 3} - 1
\]



\[
\lim\limits_{x \to \infty} H(x) = \answer{\infty}
\]



\[
\lim\limits_{x \to -\infty} H(x) = \answer{-1}
\]

\end{question}







\begin{question}



Let 

\[
H(x) = 4 2^{-5x - 3} - 1
\]


\[
\lim\limits_{x \to \infty} H(x) = \answer{-1}
\]



\[
\lim\limits_{x \to -\infty} H(x) = \answer{\infty}
\]

\end{question}





\begin{question}



Let 

\[
H(x) = -4 2^{5x - 3} - 1
\]


\[
\lim\limits_{x \to \infty} H(x) = \answer{-\infty}
\]



\[
\lim\limits_{x \to -\infty} H(x) = \answer{-1}
\]








\begin{question}



Let 

\[
H(x) = -4 2^{-5x - 3} - 1
\]


\[
\lim\limits_{x \to \infty} H(x) = \answer{-1}
\]



\[
\lim\limits_{x \to -\infty} H(x) = \answer{-\infty}
\]

\end{question}








\end{exercise}
\end{document}