\documentclass{ximera}

\input{../../preamble.tex}

\title{Operations}

\begin{document}

\begin{abstract}
addition and subtraction
\end{abstract}
\maketitle



Complex Numbers are 2-dimensional numbers, which we represent as $a + b \, i$, where $i = \sqrt{-1}$.

On one hand, $\sqrt{-1}$ is a little weird.  On the other hand, we have worked with expressions like $5 + 3 \sqrt{2}$ and $3 - 4 \sqrt{7}$ many times.  In this respect, $5 + 3 \sqrt{-1}$ is no different.  $i = \sqrt{-1}$ is simply the number you square to get $-1$.  That's all.



\begin{notation}



We have plenty of shorthand notations.

\begin{itemize}
\item $3 + 1 \, i = 3 + i$
\item $4 + 0 \, i = 4$
\item $0 + 5 \, i = 5 \, i$
\end{itemize}


\end{notation}





Addition and Subtraction are componentwise operations.


\begin{itemize}
	\item $(a + b \, i) + (c + d \, i) = (a+c) + (b+d) \, i$
	\item $(a + b \, i) - (c + d \, i) = (a-c) + (b-d) \, i$
\end{itemize}

Add the real parts. Add the imaginary parts. \\
Subtract the real parts. Subtract the imaginary parts. \\








Multiplication is a little more involved, because we want the Distributive Property.



\begin{itemize}
	\item $(a + b \, i) \cdot (c + d \, i) = (ac - bd) + (ad + bc) \, i$
\end{itemize}


\textbf{Note:}  All of this gives us our usual equivalencies, like $a + (-b) \, i = a - b \, i$

\begin{question}


\begin{itemize}
\item   $(4 + 5 \, i) + (3 + 7 \, i) = \answer{7} + \answer{12} i$
\item   $(4 + (-5) \, i) + (3 + 7 \, i) = \answer{7} + \answer{2} i$
\item   $(4 + 5 \, i) + (3 - 7 \, i) = \answer{7} + \answer{-2} i = \answer{7} - \answer{2} i$
\item   $(-4 + 5 \, i) + (3 + 7 \, i) = \answer{-1} + \answer{12} i = -\answer{1} + \answer{12} i$
\item   $(4 - 5 \, i) + (-3 + 7 \, i) = \answer{1} + \answer{2} i$
\end{itemize}



\end{question}





\begin{question}


\begin{itemize}
\item   $(4 + 5 \, i) - (3 + 7 \, i) = \answer{1} + \answer{-2} i = \answer{1} - \answer{2} i$
\item   $(4 + (-5) \, i) - (3 + 7 \, i) = \answer{1} + \answer{-12} i = \answer{1} - \answer{12} i$
\item   $(4 + 5 \, i) - (3 - 7 \, i) = \answer{1} + \answer{12} i$
\item   $(-4 + 5 \, i) - (3 + 7 \, i) = \answer{-7} + \answer{-2} i = \answer{-7} - \answer{2} i$
\item   $(4 - 5 \, i) - (-3 + 7 \, i) = \answer{7} + \answer{-12} i = \answer{7} - \answer{12} i$
\end{itemize}



\end{question}











\begin{question}


\begin{itemize}
\item   $(4 + 5 \, i) \cdot (3 + 7 \, i) = \answer{-23} + \answer{43} i$
\item   $(3 - 2 \, i) \cdot (4 + \, i) = \answer{14} + \answer{-5} i = \answer{14} - \answer{5} i$
\end{itemize}



\end{question}








\begin{question}


\begin{itemize}
\item   $(\frac{2}{3} +  \, i) + (3 + \frac{1}{2} \, i) = \answer{\frac{11}{2}} + \answer{\frac{3}{2}} i$
\item   $(\pi + (-5) \, i) + (3 - i) = \answer{3+\pi} + \answer{-6} i$
\item   $(4 + \sqrt{2} \, i) + (3 - \sqrt{2} \, i) = \answer{7}$
\item   $(-4 + \sqrt{3} \, i) + (4 + 7 \, i) = \answer{7 + \sqrt{3}} i$
\end{itemize}



\end{question}





\begin{question}


\item   $(\frac{1}{\sqrt{2}} +  \frac{1}{\sqrt{2}} \, i) \cdot (\frac{1}{\sqrt{2}} + \frac{1}{\sqrt{2}} \, i) = \answer{0} + \answer{1} i$


\end{question}










\begin{question}


\item   $(a +  b \, i) + (a - b \, i) = \answer{2a}$


\end{question}















\end{document}
