\documentclass{ximera}

\input{../../preamble.tex}

\title{Growth Rates}

\begin{document}

\begin{abstract}
constant percentage
\end{abstract}
\maketitle











The defining characteristic of linear functions is that the have a constant growth rate.


\[   \frac{f(b)-f(a)}{b-a} = m       \]

This led to the equation or formula for linear functions:  $f(x) = m(x-a) + f(a)$


This tells us that no matter where you are in the domain, of $f$, if you move a distance of $1$, the value of $f$ increases by $m$. \\


Exponential functions don't do that. \\






\begin{fact}  No Constant Growth

Let $G(t) = 5 \left(\frac{3}{2}\right)^t$ with domain \textbf{$R$}. 

$G(t) = 5 \left(\frac{3}{2}\right)^t$  does not exhibit a constant growth rate. 




\begin{itemize}
\item $G(0) = 5$
\item $G(1) = \frac{15}{2}$
\item $G(2) = \frac{45}{4}$
\end{itemize}



Each time we moved $1$ in the domain, $G(t)$ DID NOT increase by the same amount.

$G(1) - G(0) = \answer{\frac{5}{2}}$ \\

$G(2) - G(1) = \answer{\frac{15}{4}}$ \\

$ \frac{5}{2}  \ne  \frac{15}{4} $, therefore $G(t)$ does not have a constant rate-of-change. \\

\end{fact}




Instead, $G$ has a constant percentage rate-of-change. \\

No matter where you are in the domain, when you move $1$, the value of $G$ increases by the same percentage (is multiplied by the same factor).


Let $a$ be a real numbers.  The percentage rate-of-change of $G$ over the interval $[a,a+1]$ is 



\[    \frac{5 \left(\frac{3}{2}\right)^{a+1} - 5 \left(\frac{3}{2}\right)^a}{5 \left(\frac{3}{2}\right)^a}       \]


\[   \frac{5 \left(\frac{3}{2}\right)^a (\left(\frac{3}{2}\right) - 1) }{5 \left(\frac{3}{2}\right)^a}    \]


Every time we move $1$ in the domain, $G$ increases by a factor of $\frac{1}{2}$.  $G$ increases by $50\%$.





The general template for an exponential function is 

\[   exp(t) = a \, b^t   \, \text{ where } \,  a \ne 0  \, \text{ and } \,    b > 0   \]



\begin{example} Percentage Change



Let $H(t) = 3 \, 2^t$ \\

$H$ is an exponential funciton, which means it has a constant percentage change. \\

Values of $H$:

\begin{itemize}
\item $H(0) = \answer{3}$

\item $H(1) = \answer{6}$

\item $H(2) = \answer{12}$
\end{itemize}



Change in $H$:

\begin{itemize}
\item $H(1) - H(0) = \answer{3}$

\item $H(2) - H(1) = \answer{12}$

\end{itemize}





Percentage change in $H$:

\begin{itemize}
\item $\frac{H(1) - H(0)}{H(0)} = \answer{1}$, which is $\answer{100}\%$

\item $\frac{H(2) - H(1)}{H(1)} = \answer{1}$, which is $\answer{100}\%$

\end{itemize}






\end{example}



Every time $t$ increases by $1$, the value of $H$ gets multiplied by another $2$, which means its value is doubled, which means it \textbf{changes} by its current value, which means it grows by $100\%$.











\begin{example} Percentage Change



Let $k(x) = 5 \, (3/4)^x$ \\

$k$ is an exponential function, which means it has a constant percentage change. \\

Values of $k$:

\begin{itemize}
\item $k(0) = \answer{5}$

\item $k(1) = \answer{\frac{15}{4}}$

\item $k(2) = \answer{\frac{45}{16}}$
\end{itemize}



Change in $k$:

\begin{itemize}
\item $k(1) - k(0) = \answer{-\frac{5}{4}}$

\item $k(2) - k(1) = \answer{-\frac{15}{16}}$

\end{itemize}





Percentage change in $k$:

\begin{itemize}
\item $\frac{k(1) - k(0)}{k(0)} = \answer{-\frac{1}{4}}$, which is $\answer{-25}\%$

\item $\frac{k(2) - k(1)}{k(1)} = \answer{-\frac{1}{4}}$, which is $\answer{-25}\%$

\end{itemize}






\end{example}

Every time $x$ increases by $1$, the value of $k$ gets multiplied by another $\frac{3}{4}$, which means its value decreases. It loses $\frac{1}{4}$ of its value. It has a negative growth rate. It grows by $-25\%$.


















\begin{example} Percentage Change



Let $p(x) = 3 \, e^x$ \\

$p$ is an exponential funciton, which means it has a constant percentage change. \\

Values of $p$:

\begin{itemize}
\item $p(0) = 3$

\item $p(1) = 3 e$

\item $p(2) = 3 e^2$
\end{itemize}



Change in $p$:

\begin{itemize}
\item $p(1) - p(0) = 3 (e-1)$

\item $p(2) - p(1) = 3 e (e-1)$

\end{itemize}





Percentage change in $p$:

\begin{itemize}
\item $\frac{p(1) - p(0)}{p(0)} = e - 1$, which is about $171.8\%$

\item $\frac{p(2) - p(1)}{p(1)} = e-1 $, which is about $171.8\%$

\end{itemize}


\end{example}


















\begin{example} Percentage Change



Let $R(t) = a \, r^t$, with $a$ and $r$ real numbers and $r>0$ \\

$R$ is an exponential function, which means it has a constant percentage change. \\

Values of $R$:

\begin{itemize}
\item $R(0) = a$

\item $R(1) = a \, r$

\item $R(2) = a \, r^2$
\end{itemize}



Change in $R$:

\begin{itemize}
\item $R(1) - R(0) = \answer{a (r-1)}$

\item $R(2) - R(1) = \answer{a r (r-1)}$

\end{itemize}





Percentage change in $R$:

\begin{itemize}
\item $\frac{R(1) - R(0)}{R(0)} = \answer{r-1}$

\item $\frac{R(2) - R(1)}{R(1)} = \answer{r-1}$

\end{itemize}


\end{example}











\end{document}
