\documentclass{ximera}

\input{../../preamble.tex}

\title{Trig Identities}

\begin{document}

\begin{abstract}
double and half
\end{abstract}
\maketitle






\section{Double Angle Formulas}


\[   \sin(2t) = \frac{e^{i 2t} - e^{-i 2t}}{2 i}      \]


A difference of two squares.  It factors.



\[   \sin(2t) = \frac{(e^{i t} - e^{-i t})(e^{i t} + e^{-i t})}{2 i}      \]




\[   \sin(2t) = 2 \cdot \frac{(e^{i t} - e^{-i t})}{2i}    \cdot    \frac{(e^{i t} + e^{-i t})}{2}      \]



\[   \sin(2t) = 2 \sin(t)   \cos(t)      \]

This is the double angle formla for sine.











\[      \cos^2(t) - \sin^2(t)      \]



\[      \cos^2(t) - \sin^2(t)   = \left( \frac{e^{i t} + e^{-i t}}{2} \right)^2 - \left( \frac{e^{i t} - e^{-i t}}{2i} \right)^2  \]


\[      \cos^2(t) - \sin^2(t)   = \left( \frac{e^{2i t} + 2 + e^{-2i t}}{4} \right) - \left( \frac{e^{2 i t} - 2 + e^{-2i t}}{-4} \right)  \]



\[      \cos^2(t) - \sin^2(t)   = \frac{2 e^{2i t}  + 2 e^{-2i t}}{4}   = \frac{e^{2i t}  + e^{-2i t}}{2} = \cos(2t)   \]




\[      \cos^2(t) - \sin^2(t)  = \cos(2t)    \]



Additionally, we have 




\[   \cos(2t) =    \cos^2(t) - \sin^2(t)  =    \cos^2(t) - (1 - \cos^2(t)) =  2 \cos^2(t) - 1 \]


and

\[   \cos(2t) =    \cos^2(t) - \sin^2(t)  =    (1 - \sin^2(t)) - \sin^2(t)  = 1 - 2 \sin(t)     \]




































\section{Half Angle Formulas}



\[   \cos(2t)  =  2 \cos^2(t) - 1 \]


\[   \frac{1 + \cos(2t)}{2}  =   \cos^2(t)  \]



and

\[  \frac{1 -  \cos(2t)}{2}  =  \sin(t)     \]







\end{document}
