\documentclass{ximera}

\input{../../preamble.tex}

\title{Quadratic Products}

\begin{document}

\begin{abstract}
factoring
\end{abstract}
\maketitle





We have seen that there are at most two real solutions to $a \, t^2 + b \, t + c = 0$, with $a \ne 0$. 

Let's look at this from a function viewpoint.  The quadratic function  $Q(t) = a \, t^2 + b \, t + c$ has at most two real zeros.  

The quadratic formula gives explicit formulas for these roots.


\[   \frac{-b + \sqrt{b^2 - 4 a c}}{2a}     \text{ and }    \frac{-b - \sqrt{b^2 - 4 a c}}{2a}   \]



We can create another quadratic function with these two zeros.



\[ f(t) =  \left(t - \frac{-b + \sqrt{b^2 - 4 a c}}{2a}\right)   \left(t -  \frac{-b - \sqrt{b^2 - 4 a c}}{2a}\right)   \]


However, if we multiply this out, we get



\[ f(t) =   t^2 \, - \, \frac{-b + \sqrt{b^2 - 4 a c}}{2a} t \, - \, \frac{-b - \sqrt{b^2 - 4 a c}}{2a}  t \, + \, \left(\frac{-b + \sqrt{b^2 - 4 a c}}{2a}\right) \left(\frac{-b - \sqrt{b^2 - 4 a c}}{2a}\right) \]


\[ f(t) = t^2  \, - \, 2 \cdot \frac{-b}{2a} + \left(    \frac{b^2 - (b^2 - 4 a c)}{4 a^2}     \right)        \]


\[ f(t) = t^2  \, + \frac{b}{a} + \left(    \frac{4 a c}{4 a^2}     \right)        \]

\[ f(t) = t^2  \, +  \frac{b}{a} + \left(    \frac{c}{a}     \right)        \]


This quadratic function has the same two zeros.  If we multiply by $a$, we get 


\[ f(t) = a t^2 + b t + c \]

which is $Q(t)$.


We have discovered a new expression or formula for our quadratic function.



\section{Factored Form}

Every quadratic function can be written as a sum, $Q(t) = a \, t^2 + b \, t + c = 0$, with $a \ne 0$.

Every quadratic function can be written as a product, $Q(t) = (t - r_1)(t - r_2)$, where $r_1$ and $r_2$ are the real zeros, which can be obtained via the quadratic formula - provided the discrimanant is positve.  If the discriminant is $0$, then $r_1 = r_2$ and we can a square.  If the discriminant is negaqitve, then $Q(t)$ doesn't factor with real numbers.  


The process of writing the function as a product is called \textbf{factoring}. $(t - r_1)$  and $(t - r_2)$ are the \textbf{factors}.



\begin{example} \textit{Two Real Solutions} 

Factor $Q(t) = 4 t^2 - 4 t - 8$ 

The leading coefficient is $a=4$ and the quadratic formula gives us $2$ and $-1$ as zeros.  

That gives us a \textbf{factorization} of $Q(t)$:



\[    Q(t) = 4 t^2 - 4 t - 8 =  4 (t-2)(t-(-1))    = 4 (t-2)(t+1)         \]



\end{example}



The quadratic formula always works.  But, many times it is slow with lots of steps and reducing.  Sometimes it is just easier to guess the factors.



\section{Guessing Factors}


Let's begin with a quadratic function written as a sum: $g(x) = a \, x^2 + b \, x + c$.  


\textbf{Step 1:} If there are any common factors among the three terms then factor that out.


\textbf{Step 2:} We are looking for a factorization $g(x) = a \, x^2 + b \, x + c = (A \, x + B)(C \, x + D)$.

for this to happen, we need

\begin{itemize}
\item $a = A \cdot C $
\item $c = B \cdot D$
\item $b = A\cdot D + B \cdot C$
\end{itemize}

Therefore, look for pairs of factors of $a$ and pairs of factors of $c$.






\textbf{Step 3:} Step through your pairs of factors and look for $b = A \cdot D + B \cdot C$.










\begin{example} \textit{Factoring}

Factor $k(x) = 2 x^2 - 5 x - 12$.


$2$ is a prime number, therefore, it's factors are $2 \cdot 1$ or $-2 \cdot -1$.

We already know that our factorization begins as $(2 x + ?) (x + ?)$ or $(-2 x + ?) (-x + ?)$.

$-12$ factors as $-12 \cdot 1$, $12 \cdot -1$, or $-6 \cdot 2$, or  $-6 \cdot 2$, or $-4 \cdot 3$, or or $4 \cdot -3$.  Let's start stepping through our list.

Since $-5 x$ seems far away from $12$, let's skip $12$ in out list and begin stepping through our list with $-6$ and $2$.

\begin{itemize}

\item $-12 = -6 \cdot 2$ gives $(2 x + (-6)) (x + 2) = 2 x^2 - 2 x - 12$
\item $-12 = 6 \cdot -2$ gives $(2 x + 6) (x - 2) = 2 x^2 - 2 x -12$
\item $-12 = -3 \cdot 4$ gives $(2 x + (-3)) (x + 4) = 2 x^2 + 5 x - 12$
\item $-12 = 3 \cdot -4$ gives $(2 x + 3) (x + (-4)) = 2 x^2 - 5 x -12$
\end{itemize}

$2 x^2 - 5 x - 12$ factors as $(2 x + 3) (x + (-4)) = (2 x + 3)(x - 4)$

\end{example}








\begin{example} \textit{Factoring}

Factor $p(y) = 3 y^2 - 8 y - 11$.


$3$ is a prime number, therefore, it's factors are $3 \cdot 1$ or $-3 \cdot -1$. However, $-3 \cdot -1$ is actually redundant.  If we picked $-3 \cdot -1$, then we could just factor out $-1$ from both and get back to $3 \cdot 1$.


$p(y) = 3 y^2 - 8 y - 11 (3y \pm ?) (y \pm ?) $


$11$ is also a prime number. We only need to think about $11$ and $1$. And, since we need $-11$ in $p(y)$, then we know to pick opposite signs for $11$ and $1$.



\begin{itemize}
\item $(3y + 11) (y - 1) = 3 y^2 + 8 y - 11$
\end{itemize}

Everything is correct except the sign of $-8$. That tells us we are almost correct. We just need to reverse the signs.


\begin{itemize}
\item $(3y - 11) (y + 1) = 3 y^2 - 8 y - 11$
\end{itemize}





\begin{itemize}

\item $-12 = -6 \cdot 2$ gives $(2 x + (-6)) (x + 2) = 2 x^2 - 2 x - 12$
\item $-12 = 6 \cdot -2$ gives $(2 x + 6) (x - 2) = 2 x^2 - 2 x -12$
\item $-12 = -3 \cdot 4$ gives $(2 x + (-3)) (x + 4) = 2 x^2 + 5 x - 12$
\item $-12 = 3 \cdot -4$ gives $(2 x + 3) (x + (-4)) = 2 x^2 - 5 x -12$
\end{itemize}

$2 x^2 - 5 x - 12$ factors as $(2 x + 3) (x + (-4)) = (2 x + 3)(x - 4)$

\end{example}


































\end{document}
